exp: style and reorg

src/exp/core.lean
@@ -6,124 +6,25 @@ namespace tts ------------------------------------------------------------------
 
 open occurs
 
--- Grammar of expressions.
+/-- Grammar of expressions -/
 inductive exp (V : Type) : Type
-  | var  : occurs → tagged V → exp -- variable, bound or free
-  | app  : exp → exp → exp         -- function application
-  | lam  : V → exp → exp           -- lambda-abstraction
-  | let_ : V → exp → exp → exp     -- let-abstraction
-
-variables {V : Type} -- Type of variable names
+| var  : occurs → tagged V → exp -- variable, bound or free
+| app  : exp → exp → exp         -- function application
+| lam  : V → exp → exp           -- lambda-abstraction
+| let_ : V → exp → exp → exp     -- let-abstraction
 
 namespace exp ------------------------------------------------------------------
+variables {V : Type} -- Type of variable names
 
-protected
-def repr [has_repr V] : exp V → string
-  | (var bound x)  := _root_.repr x.tag ++ "⟨" ++ _root_.repr x.val ++ "⟩"
-  | (var free x)   := _root_.repr x
-  | (app ef ea)    := "(" ++ ef.repr ++ ") (" ++ ea.repr ++ ")"
-  | (lam v eb)     := "λ " ++ _root_.repr v ++ " . " ++ eb.repr
-  | (let_ v ed eb) := "let " ++ _root_.repr v ++ " = " ++ ed.repr ++ " in " ++ eb.repr
+protected def repr [has_repr V] : exp V → string
+| (var bound x)  := _root_.repr x.tag ++ "⟨" ++ _root_.repr x.val ++ "⟩"
+| (var free x)   := _root_.repr x
+| (app ef ea)    := "(" ++ ef.repr ++ ") (" ++ ea.repr ++ ")"
+| (lam v eb)     := "λ " ++ _root_.repr v ++ " . " ++ eb.repr
+| (let_ v ed eb) := "let " ++ _root_.repr v ++ " = " ++ ed.repr ++ " in " ++ eb.repr
 
 instance [has_repr V] : has_repr (exp V) :=
 ⟨exp.repr⟩
-
--- Open an expression (last parameter) with an expression (e) for a bound
--- variable.
-def open_exp (e : exp V) : ℕ → exp V → exp V
-  | k (var bound x)  := if k = x.tag then e else var bound x
-  | _ (var free x)   := var free x
-  | k (app ef ea)    := app (open_exp k ef) (open_exp k ea)
-  | k (lam v eb)     := lam v (open_exp k.succ eb)
-  | k (let_ v ed eb) := let_ v (open_exp k ed) (open_exp k.succ eb)
-
-@[simp]
-theorem open_exp_var_bound_eq {k} {x : tagged V} {e : exp V} (h : k = x.tag)
-: open_exp e k (var bound x) = e :=
-  by simp [open_exp, h]
-
-@[simp]
-theorem open_exp_var_bound_ne {k} {x : tagged V} {e : exp V} (h : k ≠ x.tag)
-: open_exp e k (var bound x) = var bound x :=
-  by simp [open_exp, h]
-
-@[simp]
-theorem open_exp_var_free {k} {x : tagged V} {e : exp V}
-: open_exp e k (var free x) = var free x :=
-  rfl
-
-@[simp]
-theorem open_exp_app {k} {e ef ea : exp V}
-: open_exp e k (app ef ea) = app (open_exp e k ef) (open_exp e k ea) :=
-  rfl
-
-@[simp]
-theorem open_exp_lam {k v} {e eb : exp V}
-: open_exp e k (lam v eb) = lam v (open_exp e k.succ eb) :=
-  rfl
-
-@[simp]
-theorem open_exp_let_ {k v} {e ed eb : exp V}
-: open_exp e k (let_ v ed eb) = let_ v (open_exp e k ed) (open_exp e k.succ eb) :=
-  rfl
-
--- Open an expression with an expression `e` for the last bound variable (0).
-def open_exp₀ (e : exp V) : exp V → exp V :=
-  open_exp e 0
-
--- Open an expression with a free variable `x` for the last bound variable.
-def open_var (x : tagged V) : exp V → exp V :=
-  open_exp₀ (var free x)
-
-variables [decidable_eq V]
-
--- Open an expression with a variable of the name `v` fresh from the variable
--- set `L` for the last bound variable.
-def open_fresh (v : V) (L : finset (tagged V)) : exp V → exp V :=
-  open_var $ (fresh.tagged v).gen L
-
--- Get the free variables of an expression
-def fv : exp V → finset (tagged V)
-  | (var bound _)  := ∅
-  | (var free x)   := {x}
-  | (app ef ea)    := fv ef ∪ fv ea
-  | (lam _ eb)     := fv eb
-  | (let_ _ ed eb) := fv ed ∪ fv eb
-
--- Substitute a free variable for an expression in an expression
-def subst (x : tagged V) (e : exp V) : exp V → exp V
-  | (var bound y)  := var bound y
-  | (var free y)   := if x = y then e else var free y
-  | (app ef ea)    := app (subst ef) (subst ea)
-  | (lam v eb)     := lam v (subst eb)
-  | (let_ v ed eb) := let_ v (subst ed) (subst eb)
-
-end /- namespace -/ exp --------------------------------------------------------
-
-namespace exp ------------------------------------------------------------------
-variables [decidable_eq V]
-
-inductive lc : exp V → Prop
-  | var  : Π x,                                                                                                    lc (var free x)
-  | app  : Π                {ef ea : exp V},              lc ef → lc ea →                                          lc (app ef ea)
-  | lam  : Π {v} (L : finset (tagged V)) {eb : exp V},            (∀ {x : tagged V}, x ∉ L → lc (open_var x eb)) → lc (lam v eb)
-  | let_ : Π {v} (L : finset (tagged V)) {ed eb : exp V}, lc ed → (∀ {x : tagged V}, x ∉ L → lc (open_var x eb)) → lc (let_ v ed eb)
-
--- Locally-closed body of a lambda- or let-expression
-def lc_body (e : exp V) : Prop :=
-  ∃ (L : finset (tagged V)), ∀ {x : tagged V}, x ∉ L → lc (open_var x e)
-
--- Grammar of values
-inductive value : exp V → Prop
-  | lam : Π {v} {e : exp V}, lc_body e → value (lam v e)
-
--- Reduction rules
-inductive red : exp V → exp V → Prop
-  | app₁  : Π {ef ef' ea : exp V},         red ef ef' → ea.lc      → red (app ef ea)         (app ef' ea)
-  | app₂  : Π {ef ea ea' : exp V},         value ef   → red ea ea' → red (app ef ea)         (app ef ea')
-  | lam   : Π {v : V} {eb ea : exp V},     lc_body eb → value ea   → red (app (lam v eb) ea) (open_exp₀ ea eb)
-  | let₁  : Π {v : V} {ed ed' eb : exp V}, red ed ed' → lc_body eb → red (let_ v ed eb)      (let_ v ed' eb)
-  | let₂  : Π {v : V} {ed eb : exp V},     value ed   → lc_body eb → red (let_ v ed eb)      (open_exp₀ ed eb)
 
 end /- namespace -/ exp --------------------------------------------------------
 end /- namespace -/ tts --------------------------------------------------------
