src/exp/fv.lean
@@ -2,39 +2,36 @@ import .core
 
 namespace tts ------------------------------------------------------------------
 namespace exp ------------------------------------------------------------------
-variables {V : Type} -- Type of variable names
+variables {V : Type} [decidable_eq V] -- Type of variable names
 variables {v : V} -- Variable names
 variables {x y : tagged V} -- Variables
 variables {ea eb ed ef : exp V} -- Expressions
 
-variables [decidable_eq V]
-
 open occurs
 
--- Properties of fv
+/-- Get the free variables of an expression -/
+def fv : exp V → finset (tagged V)
+| (var bound _)  := ∅
+| (var free x)   := {x}
+| (app ef ea)    := fv ef ∪ fv ea
+| (lam _ eb)     := fv eb
+| (let_ _ ed eb) := fv ed ∪ fv eb
 
-@[simp]
-lemma fv_var_bound : x ∉ fv (var bound y) :=
-  finset.not_mem_empty x
+@[simp] theorem fv_var_bound : x ∉ fv (var bound y) :=
+finset.not_mem_empty x
 
-@[simp]
-lemma fv_var_free : x ∉ fv (var free y) ↔ x ≠ y :=
-  ⟨ finset.not_mem_singleton.mp
-  , λ (p : x ≠ y) (h : x ∈ {y}),
-    absurd (finset.mem_of_mem_insert_of_ne h p) (finset.not_mem_empty x)
-  ⟩
+@[simp] theorem fv_var_free : x ∉ fv (var free y) ↔ x ≠ y :=
+⟨finset.not_mem_singleton.mp,
+ λ p h, absurd (finset.mem_of_mem_insert_of_ne h p) (finset.not_mem_empty x)⟩
 
-@[simp]
-lemma fv_app : x ∉ fv (app ef ea) ↔ x ∉ fv ef ∧ x ∉ fv ea :=
-  finset.not_mem_union
+@[simp] theorem fv_app : x ∉ fv (app ef ea) ↔ x ∉ fv ef ∧ x ∉ fv ea :=
+finset.not_mem_union
 
-@[simp]
-lemma fv_lam : x ∉ fv (lam v eb) ↔ x ∉ fv eb :=
-  ⟨by rw fv; exact id, by rw fv; exact id⟩
+@[simp] theorem fv_lam : x ∉ fv (lam v eb) ↔ x ∉ fv eb :=
+⟨by rw fv; exact id, by rw fv; exact id⟩
 
-@[simp]
-lemma fv_let_ : x ∉ fv (let_ v ed eb) ↔ x ∉ fv ed ∧ x ∉ fv eb :=
-  finset.not_mem_union
+@[simp] theorem fv_let_ : x ∉ fv (let_ v ed eb) ↔ x ∉ fv ed ∧ x ∉ fv eb :=
+finset.not_mem_union
 
 end /- namespace -/ exp --------------------------------------------------------
 end /- namespace -/ tts --------------------------------------------------------
