src/exp/lc.lean
@@ -1,36 +1,76 @@
-import .core
+import exp.open
 
 namespace tts ------------------------------------------------------------------
 namespace exp ------------------------------------------------------------------
-variables {V : Type} -- Type of variable names
-variables [decidable_eq V]
+variables {V : Type} [decidable_eq V] -- Type of variable names
+variables {k k₂ k₃ : ℕ} -- Natural numbers
 variables {v : V} -- Variable names
 variables {x : tagged V} -- Variables
-variables {ea eb ed ef : exp V} -- Expressions
+variables {e ea eb ed ef e₁ e₂ e₃ : exp V} -- Expressions
 
 open occurs
 
-@[simp]
-theorem lc_var (x : tagged V) : lc (var free x) :=
-  lc.var x
+/-- Locally-close expression -/
+inductive lc : exp V → Prop
+| var  : Π x,                                                                                                    lc (var free x)
+| app  : Π                {ef ea : exp V},              lc ef → lc ea →                                          lc (app ef ea)
+| lam  : Π {v} (L : finset (tagged V)) {eb : exp V},            (∀ {x : tagged V}, x ∉ L → lc (open_var x eb)) → lc (lam v eb)
+| let_ : Π {v} (L : finset (tagged V)) {ed eb : exp V}, lc ed → (∀ {x : tagged V}, x ∉ L → lc (open_var x eb)) → lc (let_ v ed eb)
 
-@[simp]
-theorem lc_app : lc (app ef ea) ↔ lc ef ∧ lc ea :=
-  ⟨ λ l, by cases l with _ _ _ l₁ l₂; exact ⟨l₁, l₂⟩
-  , λ ⟨l₁, l₂⟩, lc.app l₁ l₂
-  ⟩
+/-- Locally-closed body of a lambda- or let-expression -/
+def lc_body (e : exp V) : Prop :=
+∃ (L : finset (tagged V)), ∀ {x : tagged V}, x ∉ L → lc (open_var x e)
 
-@[simp]
-theorem lc_lam : lc (lam v eb) ↔ lc_body eb :=
-  ⟨ λ l, by cases l; apply exists.intro; assumption; assumption
-  , λ l, by cases l; apply lc.lam; assumption; assumption
-  ⟩
+@[simp] theorem lc_var (x : tagged V) : lc (var free x) :=
+lc.var x
 
-@[simp]
-theorem lc_let_ : lc (let_ v ed eb) ↔ lc ed ∧ lc_body eb :=
-  ⟨ λ l, by cases l; exact ⟨by assumption, ⟨by assumption, by assumption⟩⟩
-  , by rintro ⟨_, _, _⟩; apply lc.let_; repeat {assumption}
-  ⟩
+@[simp] theorem lc_app : lc (app ef ea) ↔ lc ef ∧ lc ea :=
+⟨λ l, by cases l with _ _ _ l₁ l₂; exact ⟨l₁, l₂⟩, λ ⟨l₁, l₂⟩, lc.app l₁ l₂⟩
+
+@[simp] theorem lc_lam : lc (lam v eb) ↔ lc_body eb :=
+⟨λ l, by cases l; apply exists.intro; assumption; assumption,
+ λ l, by cases l; apply lc.lam; assumption; assumption⟩
+
+@[simp] theorem lc_let_ : lc (let_ v ed eb) ↔ lc ed ∧ lc_body eb :=
+⟨λ l, by cases l; exact ⟨by assumption, ⟨by assumption, by assumption⟩⟩,
+ by rintro ⟨_, _, _⟩; apply lc.let_; repeat {assumption}⟩
+
+theorem open_exp_of_lc_aux (p : k₂ ≠ k₃) :
+  open_exp e₂ k₂ (open_exp e₃ k₃ e₁) = open_exp e₃ k₃ e₁ → open_exp e₂ k₂ e₁ = e₁ :=
+begin
+  induction e₁ generalizing e₂ e₃ k₂ k₃; repeat {rw open_exp},
+  case exp.var : o x {
+    cases o,
+    case occurs.bound {
+      cases x with _ i,
+      by_cases h : k₃ = i,
+      { induction h, simp [p] },
+      { simp [h] } },
+    case occurs.free { exact id }, },
+  case exp.app : ef ea ihf iha {
+    intro h,
+    injection h with hf ha,
+    conv {to_lhs, rw [ihf p hf, iha p ha]} },
+  case exp.lam : v eb rb {
+    intro h,
+    injection h with _ hb,
+    conv {to_lhs, rw rb (mt nat.succ.inj p) hb} },
+  case exp.let_ : v ed eb rd rb {
+    intro h,
+    injection h with _ hd hb,
+    conv {to_lhs, rw [rd p hd, rb (mt nat.succ.inj p) hb]} }
+end
+
+@[simp] theorem open_exp_id (l : lc e₁) : open_exp e₂ k e₁ = e₁ :=
+begin
+  induction l generalizing e₂ k; rw open_exp,
+  case lc.app : ef ea lf la rf ra { rw [rf, ra] },
+  case lc.lam : v L eb lb rb {
+    rw open_exp_of_lc_aux k.succ_ne_zero (rb ((fresh.tagged v).gen_not_mem L)) },
+  case lc.let_ : v L ed eb ld Fb rd rb {
+    rw [rd, open_exp_of_lc_aux k.succ_ne_zero (rb ((fresh.tagged v).gen_not_mem L))] }
+end
+
 
 end /- namespace -/ exp --------------------------------------------------------
 end /- namespace -/ tts --------------------------------------------------------
