src/exp/semantics.lean
@@ -1,5 +1,4 @@
-import .subst_open
-import tactics
+import tactics .subst_open
 
 namespace tts ------------------------------------------------------------------
 namespace exp ------------------------------------------------------------------
@@ -7,21 +6,33 @@ variables {V : Type} -- Type of variable names
 variables [decidable_eq V]
 variables {e₁ e₂ : exp V} -- Expressions
 
+/-- Grammar of values -/
+inductive value : exp V → Prop
+| lam : Π {v} {e : exp V}, lc_body e → value (lam v e)
+
 theorem lc_of_value : ∀ {e : exp V}, value e → lc e
-  | _ (value.lam p) := lc_lam.mpr p
+| _ (value.lam p) := lc_lam.mpr p
 
-theorem lc_of_red_left (h : red e₁ e₂) : e₁.lc :=
-  by induction h; simp [and.assoc] at *; note_all_applied lc_of_value; tauto
+/-- Reduction rules -/
+inductive red : exp V → exp V → Prop
+| app₁  : Π {ef ef' ea : exp V},     red ef ef' → ea.lc      → red (app ef ea)         (app ef' ea)
+| app₂  : Π {ef ea ea' : exp V},     value ef   → red ea ea' → red (app ef ea)         (app ef ea')
+| lam   : Π {v} {eb ea : exp V},     lc_body eb → value ea   → red (app (lam v eb) ea) (open_exp₀ ea eb)
+| let₁  : Π {v} {ed ed' eb : exp V}, red ed ed' → lc_body eb → red (let_ v ed eb)      (let_ v ed' eb)
+| let₂  : Π {v} {ed eb : exp V},     value ed   → lc_body eb → red (let_ v ed eb)      (open_exp₀ ed eb)
 
-theorem lc_of_red_right (h : red e₁ e₂) : e₂.lc :=
-  begin
-    induction h,
-    case red.app₁ { simp at *, tauto },
-    case red.app₂ { simp at *, note_all_applied lc_of_value, tauto },
-    case red.lam : v _ _ lc_eb val_ea { exact lc_open v lc_eb (lc_of_value val_ea) },
-    case red.let₁ { simp at *, tauto },
-    case red.let₂ : v _ _ val_ed lc_eb { exact lc_open v lc_eb (lc_of_value val_ed) }
-  end
+theorem lc_of_red_left (h : red e₁ e₂) : lc e₁ :=
+by induction h; simp [and.assoc] at *; note_all_applied lc_of_value; tauto
+
+theorem lc_of_red_right (h : red e₁ e₂) : lc e₂ :=
+begin
+  induction h,
+  case red.app₁ { simp at *, tauto },
+  case red.app₂ { simp at *, note_all_applied lc_of_value, tauto },
+  case red.lam : v _ _ lc_eb val_ea { exact lc_open_exp₀ v lc_eb (lc_of_value val_ea) },
+  case red.let₁ { simp at *, tauto },
+  case red.let₂ : v _ _ val_ed lc_eb { exact lc_open_exp₀ v lc_eb (lc_of_value val_ed) }
+end
 
 end /- namespace -/ exp --------------------------------------------------------
 end /- namespace -/ tts --------------------------------------------------------
