src/exp/subst.lean
@@ -10,35 +10,39 @@ variables [decidable_eq V]
 
 open occurs
 
--- Properties of subst
+/-- Substitute a free variable for an expression in an expression -/
+def subst (x : tagged V) (ex : exp V) : exp V → exp V
+| (var bound y)  := var bound y
+| (var free y)   := if x = y then ex else var free y
+| (app ef ea)    := app (subst ef) (subst ea)
+| (lam v eb)     := lam v (subst eb)
+| (let_ v ed eb) := let_ v (subst ed) (subst eb)
 
-@[simp]
-theorem subst_var_bound : subst x e (var bound y) = var bound y :=
-  rfl
+@[simp] theorem subst_var_bound : subst x ex (var bound y) = var bound y :=
+rfl
 
-@[simp]
-lemma subst_var_free_eq (h : x = y) : subst x e (var free y) = e :=
-  by simp [subst, h]
+@[simp] theorem subst_var_free_eq (h : x = y) :
+  subst x ex (var free y) = ex :=
+by simp [subst, h]
 
-@[simp]
-lemma subst_var_free_ne (h : x ≠ y) : subst x e (var free y) = var free y :=
-  by simp [subst, h]
+@[simp] theorem subst_var_free_ne (h : x ≠ y) :
+  subst x ex (var free y) = var free y :=
+by simp [subst, h]
 
-@[simp]
-lemma subst_app {ef ea : exp V} : subst x e (app ef ea) = app (subst x e ef) (subst x e ea) :=
-  rfl
+@[simp] theorem subst_app {ef ea : exp V} :
+  subst x ex (app ef ea) = app (subst x ex ef) (subst x ex ea) :=
+rfl
 
-@[simp]
-lemma subst_lam {v} {eb : exp V} : subst x e (lam v eb) = lam v (subst x e eb) :=
-  rfl
+@[simp] theorem subst_lam {v} {eb : exp V} :
+  subst x ex (lam v eb) = lam v (subst x ex eb) :=
+rfl
 
-@[simp]
-lemma subst_let_ {v} {ed eb : exp V} : subst x e (let_ v ed eb) = let_ v (subst x e ed) (subst x e eb) :=
-  rfl
+@[simp] theorem subst_let_ {v} {ed eb : exp V} :
+  subst x ex (let_ v ed eb) = let_ v (subst x ex ed) (subst x ex eb) :=
+rfl
 
-@[simp]
-lemma subst_fresh (h : x ∉ fv e) : subst x ex e = e :=
-  by induction e with o; try {cases o}; try {simp at h}; try {cases h}; simp *
+@[simp] theorem subst_fresh (h : x ∉ fv e) : subst x ex e = e :=
+by induction e with o; try {cases o}; try {simp at h}; try {cases h}; simp *
 
 end /- namespace -/ exp --------------------------------------------------------
 end /- namespace -/ tts --------------------------------------------------------
