src/exp/subst_open.lean
@@ -4,99 +4,81 @@ import .subst
 
 namespace tts ------------------------------------------------------------------
 namespace exp ------------------------------------------------------------------
+variables {V : Type} [decidable_eq V] -- Type of variable names
+variables {v : V} -- Variable names
 variables {k i : ℕ} -- Natural numbers
-variables {V : Type} -- Type of variable names
 variables {x y : tagged V} -- Variable names
 variables {e ex e₁ e₂ : exp V} -- Expressions
-
-variables [decidable_eq V]
+variables {L : finset (tagged V)} -- Variables sets
 
 open occurs
 
-@[simp]
-lemma subst_open_exp (lx : lc ex)
-: subst x ex (open_exp e₂ k e₁) = open_exp (subst x ex e₂) k (subst x ex e₁) :=
-  begin
-    induction e₁ generalizing k,
-    case exp.var : o y {
-      cases o,
-      { by_cases h : k = y.tag; simp [h] },
-      { by_cases h : x = y; simp [h, open_exp_of_lc lx] }
-    },
-    case exp.app : ef ea rf ra {
-      simp [rf, ra]
-    },
-    case exp.lam : v eb rb {
-      simp [rb]
-    },
-    case exp.let_ : v ed eb rd rb {
-      simp [rd, rb]
-    }
-  end
+@[simp] theorem subst_open_exp (lx : lc ex) :
+  subst x ex (open_exp e₂ k e₁) = open_exp (subst x ex e₂) k (subst x ex e₁) :=
+begin
+  induction e₁ generalizing k,
+  case exp.var : o y {
+    cases o,
+    { by_cases h : k = y.tag; simp [h] },
+    { by_cases h : x = y; simp [h, open_exp_id lx] } },
+  case exp.app : ef ea rf ra { simp [rf, ra] },
+  case exp.lam : v eb rb { simp [rb] },
+  case exp.let_ : v ed eb rd rb { simp [rd, rb] }
+end
 
-@[simp]
-lemma subst_open_exp₀
-: lc ex → subst x ex (open_exp₀ e₂ e₁) = open_exp₀ (subst x ex e₂) (subst x ex e₁) :=
-  subst_open_exp
+@[simp] theorem subst_open_exp₀ :
+  lc ex → subst x ex (open_exp₀ e₂ e₁) = open_exp₀ (subst x ex e₂) (subst x ex e₁) :=
+subst_open_exp
 
-@[simp]
-lemma subst_open_var (lx : lc ex) (h : x ≠ y)
-: subst x ex (open_var y e₁) = open_var y (subst x ex e₁) :=
-  by simp [open_var, h, lx]
+@[simp] theorem subst_open_var (lx : lc ex) (h : x ≠ y) :
+  subst x ex (open_var y e₁) = open_var y (subst x ex e₁) :=
+by simp [open_var, h, lx]
 
-@[simp]
-lemma subst_open_fresh {v} {L : finset (tagged V)} (lx : lc ex)
-(h : (fresh.tagged v).gen L ≠ x)
-: subst x ex (open_fresh v L e₁) = open_fresh v L (subst x ex e₁) :=
-  subst_open_var lx (ne.symm h)
+@[simp] theorem subst_open_fresh (lx : lc ex) (h : (fresh.tagged v).gen L ≠ x) :
+  subst x ex (open_fresh v L e₁) = open_fresh v L (subst x ex e₁) :=
+subst_open_var lx (ne.symm h)
 
--- subst_intro
+/- subst_intro -/
 
-lemma subst_intro
-: ∀ {e₁ : exp V} k, x ∉ fv e₁ → open_exp e₂ k e₁ = subst x e₂ (open_exp (var free x) k e₁)
-  | (var bound y)  k p := by by_cases h : k = y.tag; simp [h]
-  | (var free y)   k p := by simp at p; simp [p]
-  | (app ef ea)    k p := by simp at p; simp [subst_intro k p.1, subst_intro k p.2]
-  | (lam v eb)     k p := by simp at p; simp [subst_intro (k + 1) p]
-  | (let_ v ed eb) k p := by simp at p; simp [subst_intro k p.1, subst_intro (k + 1) p.2]
+theorem subst_intro : ∀ {e₁ : exp V} k,
+  x ∉ fv e₁ → open_exp e₂ k e₁ = subst x e₂ (open_exp (var free x) k e₁)
+| (var bound y)  k p := by by_cases h : k = y.tag; simp [h]
+| (var free y)   k p := by simp at p; simp [p]
+| (app ef ea)    k p := by simp at p; simp [subst_intro k p.1, subst_intro k p.2]
+| (lam v eb)     k p := by simp at p; simp [subst_intro (k + 1) p]
+| (let_ v ed eb) k p := by simp at p; simp [subst_intro k p.1, subst_intro (k + 1) p.2]
 
-lemma subst_intro₀ : x ∉ fv e₁ → open_exp₀ e₂ e₁ = subst x e₂ (open_var x e₁) :=
-  subst_intro 0
+theorem subst_intro₀ : x ∉ fv e₁ → open_exp₀ e₂ e₁ = subst x e₂ (open_var x e₁) :=
+subst_intro 0
 
 -- Locally-closed expressions are stable over substitution
-lemma subst_lc (x : tagged V) (lx : lc ex) (l : lc e) : lc (subst x ex e) :=
-  begin
-    induction l generalizing ex lx x,
-    case lc.var : y {
-      by_cases h : x = y; simp [h, lx]
-    },
-    case lc.app : ef ea lf la rf ra {
-      exact lc.app (rf lx x) (ra lx x)
-    },
-    case lc.lam : v L eb lb rb {
-      apply lc.lam (L ∪ {x}),
-      intros y Fy,
-      simp [not_or_distrib] at Fy,
-      rw ←subst_open_var lx (ne.symm Fy.2),
-      exact rb Fy.1 lx x
-    },
-    case lc.let_ : v L ed eb ld lb rd rb {
-      apply lc.let_ (L ∪ {x}) (rd lx x),
-      intros y Fy,
-      simp [not_or_distrib] at Fy,
-      rw ←subst_open_var lx (ne.symm Fy.2),
-      exact rb Fy.1 lx x
-    }
-  end
+theorem subst_lc (x : tagged V) (lx : lc ex) (l : lc e) : lc (subst x ex e) :=
+begin
+  induction l generalizing ex lx x,
+  case lc.var : y { by_cases h : x = y; simp [h, lx] },
+  case lc.app : ef ea lf la rf ra { exact lc.app (rf lx x) (ra lx x) },
+  case lc.lam : v L eb lb rb {
+    apply lc.lam (L ∪ {x}),
+    intros y Fy,
+    simp [not_or_distrib] at Fy,
+    rw ←subst_open_var lx (ne.symm Fy.2),
+    exact rb Fy.1 lx x },
+  case lc.let_ : v L ed eb ld lb rd rb {
+    apply lc.let_ (L ∪ {x}) (rd lx x),
+    intros y Fy,
+    simp [not_or_distrib] at Fy,
+    rw ←subst_open_var lx (ne.symm Fy.2),
+    exact rb Fy.1 lx x }
+end
 
-theorem lc_open (v : V) (lb : lc_body e₁) (l₂ : lc e₂) : lc (open_exp₀ e₂ e₁) :=
-  begin
-    cases lb with L l₁,
-    have F : (fresh.tagged v).gen (L ∪ fv e₁) ∉ L ∧ (fresh.tagged v).gen (L ∪ fv e₁) ∉ fv e₁ :=
-      (fresh.tagged v).gen_not_mem_union _ _,
-    rw subst_intro₀ F.2,
-    exact subst_lc _ l₂ (l₁ F.1)
-  end
+theorem lc_open_exp₀ (v : V) (lb : lc_body e₁) (l₂ : lc e₂) : lc (open_exp₀ e₂ e₁) :=
+begin
+  cases lb with L l₁,
+  have F : (fresh.tagged v).gen (L ∪ fv e₁) ∉ L ∧ (fresh.tagged v).gen (L ∪ fv e₁) ∉ fv e₁ :=
+    (fresh.tagged v).gen_not_mem_union _ _,
+  rw subst_intro₀ F.2,
+  exact subst_lc _ l₂ (l₁ F.1)
+end
 
 end /- namespace -/ exp --------------------------------------------------------
 end /- namespace -/ tts --------------------------------------------------------
